Rename HList -> HVector

SSA/Experimental/HVector.lean
@@ -2,11 +2,12 @@ import Mathlib.Tactic.Basic
 import Mathlib.Tactic.LibrarySearch
 
 
-inductive HList {α : Type*} (f : α → Type*) : List α → Type _
-  | nil : HList f []
-  | cons {a : α} : (f a) → HList f as → HList f (a :: as)
+/-- An heterogeneous vector -/
+inductive HVector {α : Type*} (f : α → Type*) : List α → Type _
+  | nil : HVector f []
+  | cons {a : α} : (f a) → HVector f as → HVector f (a :: as)
 
-namespace HList
+namespace HVector
 
 variable {A B : α → Type*} {as : List α}
 
@@ -14,23 +15,23 @@ variable {A B : α → Type*} {as : List α}
   # Definitions
 -/
 
-def head : HList A (a :: as) → A a
+def head : HVector A (a :: as) → A a
   | .cons x _ => x
 
-def tail : HList A (a :: as) → HList A as
+def tail : HVector A (a :: as) → HVector A as
   | .cons _ xs => xs
 
 def map (f : ∀ (a : α), A a → B a) :
-    ∀ {l : List α}, HList A l → HList B l
+    ∀ {l : List α}, HVector A l → HVector B l
   | [],   .nil        => .nil
   | t::_, .cons a as  => .cons (f t a) (map f as)
 
 def foldl {B : Type*} (f : ∀ (a : α), B → A a → B) :
-    ∀ {l : List α}, B → HList A l → B
+    ∀ {l : List α}, B → HVector A l → B
   | [],   b, .nil       => b
   | t::_, b, .cons a as => foldl f (f t b a) as
 
-def get {as} : HList A as → (i : Fin as.length) → A (as.get i)
+def get {as} : HVector A as → (i : Fin as.length) → A (as.get i)
   | .nil, i => i.elim0
   | .cons x  _, ⟨0,   _⟩  => x
   | .cons _ xs, ⟨i+1, h⟩  => get xs ⟨i, Nat.succ_lt_succ_iff.mp h⟩
@@ -42,24 +43,24 @@ def ToTupleType (A : α → Type*) : List α → Type _
   | a :: as => A a × (ToTupleType A as)
 
 /-- 
-  Turns a `HList A [a₁, a₂, ..., aₙ]` into a tuple `(A a₁) × (A a₂) × ... × (A aₙ)`
+  Turns a `HVector A [a₁, a₂, ..., aₙ]` into a tuple `(A a₁) × (A a₂) × ... × (A aₙ)`
 -/
-def toTuple {as} : HList A as → ToTupleType A as
+def toTuple {as} : HVector A as → ToTupleType A as
   | .nil => ⟨⟩
   | .cons x .nil => x
   | .cons x₁ <| .cons x₂ xs => (x₁, (cons x₂ xs).toTuple)
 
-abbrev toSingle : HList A [a₁] → A a₁ := toTuple
-abbrev toPair   : HList A [a₁, a₂] → A a₁ × A a₂ := toTuple
-abbrev toTriple : HList A [a₁, a₂, a₃] → A a₁ × A a₂ × A a₃ := toTuple
+abbrev toSingle : HVector A [a₁] → A a₁ := toTuple
+abbrev toPair   : HVector A [a₁, a₂] → A a₁ × A a₂ := toTuple
+abbrev toTriple : HVector A [a₁, a₂, a₃] → A a₁ × A a₂ × A a₃ := toTuple
 
 /-
   # Theorems
 -/
 
-theorem map_map {A B C : α → Type*} {l : List α} (t : HList A l)
+theorem map_map {A B C : α → Type*} {l : List α} (t : HVector A l)
     (f : ∀ a, A a → B a) (g : ∀ a, B a → C a) :
     (t.map f).map g = t.map (fun a v => g a (f a v)) := by
   induction t <;> simp_all [map]
 
-end HList
+end HVector
