SSA/Core/Tactic.lean
@@ -8,6 +8,6 @@ macro "simp_mlir": tactic =>
        simp (config := {decide := false}) only [TSSA.eval, Function.comp,
          id.def, TypedUserSemantics, TypedUserSemantics.eval, Context.Var,
          TypedUserSemantics.outUserType, TypedUserSemantics.argUserType,
-         UserType.mkPair, UserType.mkTriple, HList.map]
+         UserType.mkPair, UserType.mkTriple, HVector.map]
       )
    )
